u«Zµìmþ™ZŠvÚ±î¸# Tarea 3 pt 1

$$
\begin{aligned}
\dot{S} &=&-\beta S I+\alpha I \\
\dot{I} &=& \beta S I-(\gamma+d) I
\end{aligned}
$$
$$
\begin{array}{l}
\text { (1) } \dot{S}=-\beta S I+2 I \quad \dot{S}\left\{S=\alpha / \beta \frac{x}{i}=\left\{j=\frac{1}{r_0}\right.\right.\\
\frac{I=\beta S I-C Q+d) I}{h} \quad R_\theta=\frac{\beta}{a+d} \quad C=0 \quad I K I=0\\
-\beta S I+\alpha I=0\\
\left.\left.\dot{j}=-\frac{a}{\beta I S}+x I+v i N-s\right) I(\beta S)-(\alpha+d)\right)=0 \quad S=\frac{a I}{\beta R}\\
\begin{array}{ll}
\dot{i}=\beta S I-(a+d+h) I f & I=0 \\
S=0 & S=2+d) / \beta \quad S=\frac{\alpha}{\beta}
\end{array}\\
-\beta S(0)+x(0)=0 \quad S=\frac{R_0}{1} \delta \frac{1}{r_0}-\beta S+r_a+r_1=R_3 J\\
\left(\frac{a}{\beta}, 0\right) \quad \beta \frac{a+d}{\beta} I-(a+b) I=0\\
\text { S } S=\frac{\text { atd }}{\beta} \quad L(a+d)-(2+d) x=0\\
-\beta \frac{a f d}{\beta} x+2 I=0 \quad a=s=\frac{a}{\beta}\\
-I(a+d) t a d=0 \quad \beta \frac{2}{\beta} I-(a+d) I=0\\
\begin{aligned}
-I d=0 & \text { aI }-(a+s) I=0 \\
-I d=0
\end{aligned}\\
\left(\frac{1}{\pi_0}, 0\right)^{\frac{J}{1}}=0 \quad\left(\frac{a}{\beta}, 0\right)
\end{array}
$$
